HL corecursor concept; HL_ and LL_REC examples; tracing module

tests/Binder_Codatatype_Tests.thy
@@ -2,9 +2,675 @@ theory Binder_Codatatype_Tests
   imports "Binders.MRBNF_Recursor"
 begin
 
+declare [[mrbnf_internals]]
+
 binder_codatatype 'a "term" =
-Var 'a
-| App "'a term" "'a term"
-| Lam x::'a t::"'a term" binds x in t
+    Var 'a
+  | App "'a term" "'a term"
+  | Lam x::'a t::"'a term" binds x in t
+
+lemmas case_sum_if =
+  if_distrib[of "case_sum f g" _ "Inl x" "Inr y", unfolded sum.case] for f g x y
+
+locale HL_COREC_term =
+  fixes is_Udvar    :: "'u \<Rightarrow> bool"
+    and Udvar       :: "'u \<Rightarrow> 'a :: covar"
+    and is_Udapp    :: "'u \<Rightarrow> bool"
+    and Udapp_stop1 :: "'u \<Rightarrow> bool"
+    and Udapp_end1  :: "'u \<Rightarrow> 'a term"
+    and Udapp_cont1 :: "'u \<Rightarrow> 'u"
+    and Udapp_stop2 :: "'u \<Rightarrow> bool"
+    and Udapp_end2  :: "'u \<Rightarrow> 'a term"
+    and Udapp_cont2 :: "'u \<Rightarrow> 'u"
+    and is_Udlam    :: "'u \<Rightarrow> bool"
+    and Udlam_stop  :: "'u \<Rightarrow> bool"
+    and Udlam_end   :: "'u \<Rightarrow> ('a \<times> 'a term) set"
+    and Udlam_cont  :: "'u \<Rightarrow> ('a \<times> 'u) set"
+    and Umap        :: "('a \<Rightarrow> 'a) \<Rightarrow> 'u \<Rightarrow> 'u"
+    and UFVars      :: "'u \<Rightarrow> 'a set"
+    and validU      :: "'u \<Rightarrow> bool"
+  assumes
+    ctor_partition: "\<And>d. validU d \<Longrightarrow>
+        (is_Udvar d \<and> \<not> is_Udapp d \<and> \<not> is_Udlam d) \<or>
+        (\<not> is_Udvar d \<and> is_Udapp d \<and> \<not> is_Udlam d) \<or>
+        (\<not> is_Udvar d \<and> \<not> is_Udapp d \<and> is_Udlam d)"
+    and Udlam_end_ne:
+      "\<And>d. validU d \<Longrightarrow> is_Udlam d \<Longrightarrow> Udlam_stop d \<Longrightarrow> Udlam_end d \<noteq> {}"
+    and Udlam_cont_ne:
+      "\<And>d. validU d \<Longrightarrow> is_Udlam d \<Longrightarrow> \<not> Udlam_stop d \<Longrightarrow> Udlam_cont d \<noteq> {}"
+    and Udlam_end_alpha:
+      "\<And>d x t x' t'. validU d \<Longrightarrow> is_Udlam d \<Longrightarrow> Udlam_stop d \<Longrightarrow>
+       (x, t) \<in> Udlam_end d \<Longrightarrow> (x', t') \<in> Udlam_end d \<Longrightarrow>
+       \<exists>f. bij f \<and> |supp f| <o |UNIV :: 'a set| \<and>
+           id_on (set_term t - {x}) f \<and> f x = x' \<and> permute_term f t = t'"
+    and Udlam_cont_alpha:
+      "\<And>d x u x' u'. validU d \<Longrightarrow> is_Udlam d \<Longrightarrow> \<not> Udlam_stop d \<Longrightarrow>
+       (x, u) \<in> Udlam_cont d \<Longrightarrow> (x', u') \<in> Udlam_cont d \<Longrightarrow>
+       \<exists>f. bij f \<and> |supp f| <o |UNIV :: 'a set| \<and>
+           id_on (UFVars u - {x}) f \<and> f x = x' \<and> Umap f u = u'"
+    and UFVars_Udvar:
+      "\<And>d. validU d \<Longrightarrow> is_Udvar d \<Longrightarrow> Udvar d \<in> UFVars d"
+    and UFVars_Udapp_end1:
+      "\<And>d. validU d \<Longrightarrow> is_Udapp d \<Longrightarrow> Udapp_stop1 d \<Longrightarrow>
+       set_term (Udapp_end1 d) \<subseteq> UFVars d"
+    and UFVars_Udapp_cont1:
+      "\<And>d. validU d \<Longrightarrow> is_Udapp d \<Longrightarrow> \<not> Udapp_stop1 d \<Longrightarrow>
+       UFVars (Udapp_cont1 d) \<subseteq> UFVars d"
+    and UFVars_Udapp_end2:
+      "\<And>d. validU d \<Longrightarrow> is_Udapp d \<Longrightarrow> Udapp_stop2 d \<Longrightarrow>
+       set_term (Udapp_end2 d) \<subseteq> UFVars d"
+    and UFVars_Udapp_cont2:
+      "\<And>d. validU d \<Longrightarrow> is_Udapp d \<Longrightarrow> \<not> Udapp_stop2 d \<Longrightarrow>
+       UFVars (Udapp_cont2 d) \<subseteq> UFVars d"
+    and UFVars_Udlam_end:
+      "\<And>d x t. validU d \<Longrightarrow> is_Udlam d \<Longrightarrow> Udlam_stop d \<Longrightarrow>
+       (x, t) \<in> Udlam_end d \<Longrightarrow> set_term t - {x} \<subseteq> UFVars d"
+    and UFVars_Udlam_cont:
+      "\<And>d x u. validU d \<Longrightarrow> is_Udlam d \<Longrightarrow> \<not> Udlam_stop d \<Longrightarrow>
+       (x, u) \<in> Udlam_cont d \<Longrightarrow> UFVars u - {x} \<subseteq> UFVars d"
+    and Umap_is_Udvar:
+      "\<And>d f. validU d \<Longrightarrow> bij f \<Longrightarrow> |supp f| <o |UNIV :: 'a set| \<Longrightarrow>
+       is_Udvar (Umap f d) \<longleftrightarrow> is_Udvar d"
+    and Umap_is_Udapp:
+      "\<And>d f. validU d \<Longrightarrow> bij f \<Longrightarrow> |supp f| <o |UNIV :: 'a set| \<Longrightarrow>
+       is_Udapp (Umap f d) \<longleftrightarrow> is_Udapp d"
+    and Umap_is_Udlam:
+      "\<And>d f. validU d \<Longrightarrow> bij f \<Longrightarrow> |supp f| <o |UNIV :: 'a set| \<Longrightarrow>
+       is_Udlam (Umap f d) \<longleftrightarrow> is_Udlam d"
+    and Umap_Udapp_stop1:
+      "\<And>d f. validU d \<Longrightarrow> bij f \<Longrightarrow> |supp f| <o |UNIV :: 'a set| \<Longrightarrow>
+       is_Udapp d \<Longrightarrow> Udapp_stop1 (Umap f d) \<longleftrightarrow> Udapp_stop1 d"
+    and Umap_Udapp_stop2:
+      "\<And>d f. validU d \<Longrightarrow> bij f \<Longrightarrow> |supp f| <o |UNIV :: 'a set| \<Longrightarrow>
+       is_Udapp d \<Longrightarrow> Udapp_stop2 (Umap f d) \<longleftrightarrow> Udapp_stop2 d"
+    and Umap_Udlam_stop:
+      "\<And>d f. validU d \<Longrightarrow> bij f \<Longrightarrow> |supp f| <o |UNIV :: 'a set| \<Longrightarrow>
+       is_Udlam d \<Longrightarrow> Udlam_stop (Umap f d) \<longleftrightarrow> Udlam_stop d"
+    and Umap_Udvar:
+      "\<And>d f. validU d \<Longrightarrow> bij f \<Longrightarrow> |supp f| <o |UNIV :: 'a set| \<Longrightarrow>
+       is_Udvar d \<Longrightarrow> Udvar (Umap f d) = f (Udvar d)"
+    and Umap_Udapp_end1:
+      "\<And>d f. validU d \<Longrightarrow> bij f \<Longrightarrow> |supp f| <o |UNIV :: 'a set| \<Longrightarrow>
+       is_Udapp d \<Longrightarrow> Udapp_stop1 d \<Longrightarrow>
+       Udapp_end1 (Umap f d) = permute_term f (Udapp_end1 d)"
+    and Umap_Udapp_cont1:
+      "\<And>d f. validU d \<Longrightarrow> bij f \<Longrightarrow> |supp f| <o |UNIV :: 'a set| \<Longrightarrow>
+       is_Udapp d \<Longrightarrow> \<not> Udapp_stop1 d \<Longrightarrow>
+       Udapp_cont1 (Umap f d) = Umap f (Udapp_cont1 d)"
+    and Umap_Udapp_end2:
+      "\<And>d f. validU d \<Longrightarrow> bij f \<Longrightarrow> |supp f| <o |UNIV :: 'a set| \<Longrightarrow>
+       is_Udapp d \<Longrightarrow> Udapp_stop2 d \<Longrightarrow>
+       Udapp_end2 (Umap f d) = permute_term f (Udapp_end2 d)"
+    and Umap_Udapp_cont2:
+      "\<And>d f. validU d \<Longrightarrow> bij f \<Longrightarrow> |supp f| <o |UNIV :: 'a set| \<Longrightarrow>
+       is_Udapp d \<Longrightarrow> \<not> Udapp_stop2 d \<Longrightarrow>
+       Udapp_cont2 (Umap f d) = Umap f (Udapp_cont2 d)"
+    and Umap_Udlam_end:
+      "\<And>d f. validU d \<Longrightarrow> bij f \<Longrightarrow> |supp f| <o |UNIV :: 'a set| \<Longrightarrow>
+       is_Udlam d \<Longrightarrow> Udlam_stop d \<Longrightarrow>
+       Udlam_end (Umap f d) = (\<lambda>(x, t). (f x, permute_term f t)) ` Udlam_end d"
+    and Umap_Udlam_cont:
+      "\<And>d f. validU d \<Longrightarrow> bij f \<Longrightarrow> |supp f| <o |UNIV :: 'a set| \<Longrightarrow>
+       is_Udlam d \<Longrightarrow> \<not> Udlam_stop d \<Longrightarrow>
+       Udlam_cont (Umap f d) = (\<lambda>(x, u). (f x, Umap f u)) ` Udlam_cont d"
+    and validU_Udapp_cont1:
+      "\<And>d. validU d \<Longrightarrow> is_Udapp d \<Longrightarrow> \<not> Udapp_stop1 d \<Longrightarrow>
+       validU (Udapp_cont1 d)"
+    and validU_Udapp_cont2:
+      "\<And>d. validU d \<Longrightarrow> is_Udapp d \<Longrightarrow> \<not> Udapp_stop2 d \<Longrightarrow>
+       validU (Udapp_cont2 d)"
+    and validU_Udlam_cont:
+      "\<And>d x u. validU d \<Longrightarrow> is_Udlam d \<Longrightarrow> \<not> Udlam_stop d \<Longrightarrow>
+       (x, u) \<in> Udlam_cont d \<Longrightarrow> validU u"
+    and Umap_comp:
+      "\<And>d f g. validU d \<Longrightarrow>
+       bij f \<Longrightarrow> |supp f| <o |UNIV :: 'a set| \<Longrightarrow>
+       bij g \<Longrightarrow> |supp g| <o |UNIV :: 'a set| \<Longrightarrow>
+       Umap f (Umap g d) = Umap (f \<circ> g) d"
+    and Umap_cong_id:
+      "\<And>d f. validU d \<Longrightarrow>
+       bij f \<Longrightarrow> |supp f| <o |UNIV :: 'a set| \<Longrightarrow>
+       (\<And>a. a \<in> UFVars d \<Longrightarrow> f a = a) \<Longrightarrow> Umap f d = d"
+    and validU_Umap:
+      "\<And>d f. validU d \<Longrightarrow>
+       bij f \<Longrightarrow> |supp f| <o |UNIV :: 'a set| \<Longrightarrow>
+       validU (Umap f d)"
+begin
+
+definition Udtor :: "'u \<Rightarrow> ('a, 'a, 'a term + 'u, 'a term + 'u) term_pre set" where
+  "Udtor d =
+    (if is_Udvar d then {Abs_term_pre (Inl (Udvar d))}
+     else if is_Udapp d then
+       {Abs_term_pre (Inr (Inl
+         ((if Udapp_stop1 d then Inl (Udapp_end1 d) else Inr (Udapp_cont1 d)),
+          (if Udapp_stop2 d then Inl (Udapp_end2 d) else Inr (Udapp_cont2 d)))))}
+     else if is_Udlam d \<and> Udlam_stop d then
+       (\<lambda>(x, t). Abs_term_pre (Inr (Inr (x, Inl t)))) ` Udlam_end d
+     else if is_Udlam d \<and> \<not> Udlam_stop d then
+       (\<lambda>(x, u). Abs_term_pre (Inr (Inr (x, Inr u)))) ` Udlam_cont d
+     else {})"
+
+(* Consequences of the constructor partition *)
+
+lemma is_Udapp_not_Udvar: "validU d \<Longrightarrow> is_Udapp d \<Longrightarrow> \<not> is_Udvar d"
+  apply (drule ctor_partition)
+  apply (elim disjE conjE)
+    apply ((erule notE, assumption) | assumption)+
+  done
+
+lemma is_Udlam_not_Udvar: "validU d \<Longrightarrow> is_Udlam d \<Longrightarrow> \<not> is_Udvar d"
+  apply (drule ctor_partition)
+  apply (elim disjE conjE)
+    apply ((erule notE, assumption) | assumption)+
+  done
+
+lemma is_Udlam_not_Udapp: "validU d \<Longrightarrow> is_Udlam d \<Longrightarrow> \<not> is_Udapp d"
+  apply (drule ctor_partition)
+  apply (elim disjE conjE)
+    apply ((erule notE, assumption) | assumption)+
+  done
+
+(* Case characterisations of Udtor *)
+
+lemma Udtor_Udvar:
+  "validU d \<Longrightarrow> is_Udvar d \<Longrightarrow>
+   Udtor d = {Abs_term_pre (Inl (Udvar d))}"
+  unfolding Udtor_def
+  apply (rule if_P, assumption)
+  done
+
+lemma Udtor_Udapp:
+  "validU d \<Longrightarrow> is_Udapp d \<Longrightarrow>
+   Udtor d = {Abs_term_pre (Inr (Inl
+     ((if Udapp_stop1 d then Inl (Udapp_end1 d) else Inr (Udapp_cont1 d)),
+      (if Udapp_stop2 d then Inl (Udapp_end2 d) else Inr (Udapp_cont2 d)))))}"
+  unfolding Udtor_def
+  apply (rule trans[OF if_not_P])
+   apply (rule is_Udapp_not_Udvar, assumption+)
+  apply (rule if_P, assumption)
+  done
+
+lemma Udtor_Udlam_stop:
+  "validU d \<Longrightarrow> is_Udlam d \<Longrightarrow> Udlam_stop d \<Longrightarrow>
+   Udtor d = (\<lambda>(x, t). Abs_term_pre (Inr (Inr (x, Inl t)))) ` Udlam_end d"
+  unfolding Udtor_def
+  apply (rule trans[OF if_not_P])
+   apply (rule is_Udlam_not_Udvar, assumption+)
+  apply (rule trans[OF if_not_P])
+   apply (rule is_Udlam_not_Udapp, assumption+)
+  apply (rule if_P, rule conjI, assumption+)
+  done
+
+lemma Udtor_Udlam_cont:
+  "validU d \<Longrightarrow> is_Udlam d \<Longrightarrow> \<not> Udlam_stop d \<Longrightarrow>
+   Udtor d = (\<lambda>(x, u). Abs_term_pre (Inr (Inr (x, Inr u)))) ` Udlam_cont d"
+  unfolding Udtor_def
+  apply (rule trans[OF if_not_P])
+   apply (rule is_Udlam_not_Udvar, assumption+)
+  apply (rule trans[OF if_not_P])
+   apply (rule is_Udlam_not_Udapp, assumption+)
+  apply (rule trans[OF if_not_P])
+   apply (rule contrapos_nn[of "Udlam_stop d"], assumption, erule conjunct2)
+  apply (rule if_P, rule conjI, assumption+)
+  done
+
+(* Properties of the App argument summands *)
+
+lemma UFVars_Udapp_if1:
+  "validU d \<Longrightarrow> is_Udapp d \<Longrightarrow>
+   case_sum set_term UFVars
+     (if Udapp_stop1 d then Inl (Udapp_end1 d) else Inr (Udapp_cont1 d)) \<subseteq> UFVars d"
+  apply (cases "Udapp_stop1 d")
+   apply (subst if_P, assumption)
+   apply (unfold sum.case)
+   apply (rule UFVars_Udapp_end1, assumption+)
+  apply (subst if_not_P, assumption)
+  apply (unfold sum.case)
+  apply (rule UFVars_Udapp_cont1, assumption+)
+  done
+
+lemma UFVars_Udapp_if2:
+  "validU d \<Longrightarrow> is_Udapp d \<Longrightarrow>
+   case_sum set_term UFVars
+     (if Udapp_stop2 d then Inl (Udapp_end2 d) else Inr (Udapp_cont2 d)) \<subseteq> UFVars d"
+  apply (cases "Udapp_stop2 d")
+   apply (subst if_P, assumption)
+   apply (unfold sum.case)
+   apply (rule UFVars_Udapp_end2, assumption+)
+  apply (subst if_not_P, assumption)
+  apply (unfold sum.case)
+  apply (rule UFVars_Udapp_cont2, assumption+)
+  done
+
+lemma validU_Udapp_if1:
+  "validU d \<Longrightarrow> is_Udapp d \<Longrightarrow>
+   pred_sum (\<lambda>_. True) validU
+     (if Udapp_stop1 d then Inl (Udapp_end1 d) else Inr (Udapp_cont1 d))"
+  apply (cases "Udapp_stop1 d")
+   apply (subst if_P, assumption)
+   apply (unfold pred_sum_inject)
+   apply (rule TrueI)
+  apply (subst if_not_P, assumption)
+  apply (unfold pred_sum_inject)
+  apply (rule validU_Udapp_cont1, assumption+)
+  done
+
+lemma validU_Udapp_if2:
+  "validU d \<Longrightarrow> is_Udapp d \<Longrightarrow>
+   pred_sum (\<lambda>_. True) validU
+     (if Udapp_stop2 d then Inl (Udapp_end2 d) else Inr (Udapp_cont2 d))"
+  apply (cases "Udapp_stop2 d")
+   apply (subst if_P, assumption)
+   apply (unfold pred_sum_inject)
+   apply (rule TrueI)
+  apply (subst if_not_P, assumption)
+  apply (unfold pred_sum_inject)
+  apply (rule validU_Udapp_cont2, assumption+)
+  done
+
+lemma Umap_Udapp_if1:
+  "validU d \<Longrightarrow> bij f \<Longrightarrow> |supp f| <o |UNIV :: 'a set| \<Longrightarrow> is_Udapp d \<Longrightarrow>
+   (if Udapp_stop1 (Umap f d) then Inl (Udapp_end1 (Umap f d))
+    else Inr (Udapp_cont1 (Umap f d))) =
+   map_sum (permute_term f) (Umap f)
+     (if Udapp_stop1 d then Inl (Udapp_end1 d) else Inr (Udapp_cont1 d))"
+  apply (cases "Udapp_stop1 d")
+   apply (subst if_P)
+    apply (rule Umap_Udapp_stop1[THEN iffD2], assumption+)
+   apply (subst if_P, assumption)
+   apply (unfold map_sum.simps)
+   apply (rule arg_cong[of _ _ Inl])
+   apply (rule Umap_Udapp_end1, assumption+)
+  apply (subst if_not_P)
+   apply (rule contrapos_nn[of "Udapp_stop1 d"], assumption)
+   apply (rule Umap_Udapp_stop1[THEN iffD1], assumption+)
+  apply (subst if_not_P, assumption)
+  apply (unfold map_sum.simps)
+  apply (rule arg_cong[of _ _ Inr])
+  apply (rule Umap_Udapp_cont1, assumption+)
+  done
+
+lemma Umap_Udapp_if2:
+  "validU d \<Longrightarrow> bij f \<Longrightarrow> |supp f| <o |UNIV :: 'a set| \<Longrightarrow> is_Udapp d \<Longrightarrow>
+   (if Udapp_stop2 (Umap f d) then Inl (Udapp_end2 (Umap f d))
+    else Inr (Udapp_cont2 (Umap f d))) =
+   map_sum (permute_term f) (Umap f)
+     (if Udapp_stop2 d then Inl (Udapp_end2 d) else Inr (Udapp_cont2 d))"
+  apply (cases "Udapp_stop2 d")
+   apply (subst if_P)
+    apply (rule Umap_Udapp_stop2[THEN iffD2], assumption+)
+   apply (subst if_P, assumption)
+   apply (unfold map_sum.simps)
+   apply (rule arg_cong[of _ _ Inl])
+   apply (rule Umap_Udapp_end2, assumption+)
+  apply (subst if_not_P)
+   apply (rule contrapos_nn[of "Udapp_stop2 d"], assumption)
+   apply (rule Umap_Udapp_stop2[THEN iffD1], assumption+)
+  apply (subst if_not_P, assumption)
+  apply (unfold map_sum.simps)
+  apply (rule arg_cong[of _ _ Inr])
+  apply (rule Umap_Udapp_cont2, assumption+)
+  done
+
+(* Factored unfold blocks *)
+
+lemmas term_pre_map_simps =
+  map_term_pre_def comp_def Abs_term_pre_inverse[OF UNIV_I]
+  map_sum.simps map_prod_simp sum.case prod.case
+  fst_conv snd_conv id_apply
+
+lemmas term_pre_set_simps =
+  set1_term_pre_def set2_term_pre_def set3_term_pre_def set4_term_pre_def
+  comp_def Abs_term_pre_inverse[OF UNIV_I]
+  map_sum.simps map_prod_simp sum_set_simps prod_set_simps sum.case
+  image_insert image_empty image_Un
+  Union_insert Union_empty Union_Un_distrib
+  Un_empty_left Un_empty_right
+  empty_Diff Diff_empty
+
+lemmas ball_unfolds = ball_Un ball_simps simp_thms
+
+interpretation HL_to_LL: COREC_term Udtor Umap UFVars validU
+  apply unfold_locales
+
+  (* Udtor_ne *)
+  subgoal for d
+    apply (frule ctor_partition)
+    apply (elim disjE conjE)
+      apply (subst Udtor_Udvar, assumption+)
+      apply (rule insert_not_empty)
+     apply (subst Udtor_Udapp, assumption+)
+     apply (rule insert_not_empty)
+    apply (cases "Udlam_stop d")
+     apply (subst Udtor_Udlam_stop, assumption+)
+     apply (unfold image_is_empty)
+     apply (rule Udlam_end_ne, assumption+)
+    apply (subst Udtor_Udlam_cont, assumption+)
+    apply (unfold image_is_empty)
+    apply (rule Udlam_cont_ne, assumption+)
+    done
+
+  (* alpha_Udtor *)
+  subgoal for X X' d
+    apply (frule ctor_partition)
+    apply (elim disjE conjE)
+      subgoal
+        apply (subst (asm) Udtor_Udvar, assumption+)
+        apply (unfold insert_subset singleton_iff)
+        apply ((erule conjE)+)?
+        apply hypsubst_thin
+        apply (rule exI[where x=id])
+        apply (rule conjI bij_id supp_id_bound id_on_id)+
+        apply (unfold term_pre_map_simps)
+        apply (rule refl)
+        done
+     subgoal
+       apply (subst (asm) Udtor_Udapp, assumption+)
+       apply (unfold insert_subset singleton_iff)
+       apply ((erule conjE)+)?
+       apply hypsubst_thin
+       apply (rule exI[where x=id])
+       apply (rule conjI bij_id supp_id_bound id_on_id)+
+       apply (unfold term_pre_map_simps)
+       apply (rule refl)
+       done
+    apply (cases "Udlam_stop d")
+     subgoal
+       apply (subst (asm) Udtor_Udlam_stop, assumption+)
+       apply (unfold insert_subset)
+       apply ((erule conjE)+)?
+       apply (erule imageE)+
+       apply hypsubst_thin
+       subgoal for p p'
+         apply (cases p)
+         apply (cases p')
+         apply hypsubst_thin
+         apply (unfold prod.case)
+         subgoal for x t x' t'
+           apply (unfold term_pre_set_simps)
+           apply (frule Udlam_end_alpha[of _ x t x' t'], assumption+)
+           apply (erule exE)
+           apply ((erule conjE)+)?
+           apply hypsubst_thin
+           apply (rule exI)
+           apply ((rule conjI, assumption)+)
+           apply (unfold term_pre_map_simps)
+           apply (rule refl)
+           done
+         done
+       done
+    subgoal
+      apply (subst (asm) Udtor_Udlam_cont, assumption+)
+      apply (unfold insert_subset)
+      apply ((erule conjE)+)?
+      apply (erule imageE)+
+      apply hypsubst_thin
+      subgoal for p p'
+        apply (cases p)
+        apply (cases p')
+        apply hypsubst_thin
+        apply (unfold prod.case)
+        subgoal for x u x' u'
+          apply (unfold term_pre_set_simps)
+          apply (frule Udlam_cont_alpha[of _ x u x' u'], assumption+)
+          apply (erule exE)
+          apply ((erule conjE)+)?
+          apply hypsubst_thin
+          apply (rule exI)
+          apply ((rule conjI, assumption)+)
+          apply (unfold term_pre_map_simps)
+          apply (rule refl)
+          done
+        done
+      done
+    done
+
+  (* UFVars_Udtor *)
+  subgoal for d X
+    apply (frule ctor_partition)
+    apply (elim disjE conjE)
+      subgoal
+        apply (subst (asm) Udtor_Udvar, assumption+)
+        apply (drule singletonD)
+        apply hypsubst_thin
+        apply (unfold term_pre_set_simps insert_subset)
+        apply (rule conjI)
+         apply (rule UFVars_Udvar, assumption+)
+        apply (rule empty_subsetI)
+        done
+     subgoal
+       apply (subst (asm) Udtor_Udapp, assumption+)
+       apply (drule singletonD)
+       apply hypsubst_thin
+       apply (unfold term_pre_set_simps)
+       apply (rule Un_least)
+        apply (rule UFVars_Udapp_if1, assumption+)
+       apply (rule UFVars_Udapp_if2, assumption+)
+       done
+    apply (cases "Udlam_stop d")
+     subgoal
+       apply (subst (asm) Udtor_Udlam_stop, assumption+)
+       apply (erule imageE)
+       apply hypsubst_thin
+       subgoal for p
+         apply (cases p)
+         apply hypsubst_thin
+         apply (unfold prod.case term_pre_set_simps)
+         apply (rule UFVars_Udlam_end, assumption+)
+         done
+       done
+    subgoal
+      apply (subst (asm) Udtor_Udlam_cont, assumption+)
+      apply (erule imageE)
+      apply hypsubst_thin
+      subgoal for p
+        apply (cases p)
+        apply hypsubst_thin
+        apply (unfold prod.case term_pre_set_simps)
+        apply (rule UFVars_Udlam_cont, assumption+)
+        done
+      done
+    done
+
+  (* Umap_Udtor *)
+  subgoal for f d
+    apply (frule ctor_partition)
+    apply (elim disjE conjE)
+      subgoal
+        apply (subst Udtor_Udvar)
+          apply (rule validU_Umap, assumption+)
+         apply (rule Umap_is_Udvar[THEN iffD2], assumption+)
+        apply (subst Udtor_Udvar, assumption+)
+        apply (subst Umap_Udvar, assumption+)
+        apply (unfold image_insert image_empty term_pre_map_simps)
+        apply (rule subset_refl)
+        done
+     subgoal
+       apply (subst Udtor_Udapp)
+         apply (rule validU_Umap, assumption+)
+        apply (rule Umap_is_Udapp[THEN iffD2], assumption+)
+       apply (subst Udtor_Udapp, assumption+)
+       apply (subst Umap_Udapp_if1, assumption+)
+       apply (subst Umap_Udapp_if2, assumption+)
+       apply (unfold image_insert image_empty term_pre_map_simps)
+       apply (rule subset_refl)
+       done
+    apply (cases "Udlam_stop d")
+     subgoal
+       apply (subst Udtor_Udlam_stop)
+          apply (rule validU_Umap, assumption+)
+         apply (rule Umap_is_Udlam[THEN iffD2], assumption+)
+        apply (rule Umap_Udlam_stop[THEN iffD2], assumption+)
+       apply (subst Udtor_Udlam_stop, assumption+)
+       apply (subst Umap_Udlam_end, assumption+)
+       apply (unfold image_image split_beta term_pre_map_simps)
+       apply (rule subset_refl)
+       done
+    subgoal
+      apply (subst Udtor_Udlam_cont)
+         apply (rule validU_Umap, assumption+)
+        apply (rule Umap_is_Udlam[THEN iffD2], assumption+)
+       apply (rule contrapos_nn[of "Udlam_stop d"], assumption)
+       apply (rule Umap_Udlam_stop[THEN iffD1], assumption+)
+      apply (subst Udtor_Udlam_cont, assumption+)
+      apply (subst Umap_Udlam_cont, assumption+)
+      apply (unfold image_image split_beta term_pre_map_simps)
+      apply (rule subset_refl)
+      done
+    done
+
+  apply (rule Umap_comp; assumption)
+   apply (rule Umap_cong_id; assumption)
+  apply (rule validU_Umap; assumption)
+
+  (* valid_Udtor *)
+  subgoal for d X
+    apply (frule ctor_partition)
+    apply (elim disjE conjE)
+      subgoal
+        apply (subst (asm) Udtor_Udvar, assumption+)
+        apply (drule singletonD)
+        apply hypsubst_thin
+        apply (unfold term_pre.pred_set term_pre_set_simps ball_unfolds)
+        apply (rule TrueI)
+        done
+     subgoal
+       apply (subst (asm) Udtor_Udapp, assumption+)
+       apply (drule singletonD)
+       apply hypsubst_thin
+       apply (unfold term_pre.pred_set term_pre_set_simps ball_unfolds)
+       apply (rule conjI)
+        apply (rule validU_Udapp_if1, assumption+)
+       apply (rule validU_Udapp_if2, assumption+)
+       done
+    apply (cases "Udlam_stop d")
+     subgoal
+       apply (subst (asm) Udtor_Udlam_stop, assumption+)
+       apply (erule imageE)
+       apply hypsubst_thin
+       subgoal for p
+         apply (cases p)
+         apply hypsubst_thin
+         apply (unfold prod.case term_pre.pred_set term_pre_set_simps ball_unfolds
+                  pred_sum_inject)
+         apply (rule TrueI)
+         done
+       done
+    subgoal
+      apply (subst (asm) Udtor_Udlam_cont, assumption+)
+      apply (erule imageE)
+      apply hypsubst_thin
+      subgoal for p
+        apply (cases p)
+        apply hypsubst_thin
+        apply (unfold prod.case term_pre.pred_set term_pre_set_simps ball_unfolds
+                 pred_sum_inject)
+        apply (rule validU_Udlam_cont, assumption+)
+        done
+      done
+    done
+  done
+
+definition HL_COREC_term :: "'u \<Rightarrow> 'a term" where
+  "HL_COREC_term = HL_to_LL.COREC_term"
+
+lemma HL_COREC_term_Var:
+  "validU u \<Longrightarrow> is_Udvar u \<Longrightarrow> HL_COREC_term u = Var (Udvar u)"
+  unfolding HL_COREC_term_def Var_def
+  apply (subst HL_to_LL.COREC_dtor[of "Abs_term_pre (Inl (Udvar u))"])
+    apply (subst Udtor_Udvar, assumption+)
+    apply (rule insertI1)
+   apply assumption
+  apply (unfold term_pre_map_simps)
+  apply (rule refl)
+  done
+
+lemma HL_COREC_term_App:
+  "validU u \<Longrightarrow> is_Udapp u \<Longrightarrow>
+   HL_COREC_term u =
+     App (if Udapp_stop1 u then Udapp_end1 u else HL_COREC_term (Udapp_cont1 u))
+         (if Udapp_stop2 u then Udapp_end2 u else HL_COREC_term (Udapp_cont2 u))"
+  unfolding HL_COREC_term_def App_def
+  apply (subst HL_to_LL.COREC_dtor[of
+    "Abs_term_pre (Inr (Inl
+       ((if Udapp_stop1 u then Inl (Udapp_end1 u) else Inr (Udapp_cont1 u)),
+        (if Udapp_stop2 u then Inl (Udapp_end2 u) else Inr (Udapp_cont2 u)))))"])
+    apply (subst Udtor_Udapp, assumption+)
+    apply (rule insertI1)
+   apply assumption
+  apply (unfold term_pre_map_simps case_sum_if)
+  apply (rule refl)
+  done
+
+lemma HL_COREC_term_Lam_stop:
+  "validU u \<Longrightarrow> is_Udlam u \<Longrightarrow> Udlam_stop u \<Longrightarrow> (x, t) \<in> Udlam_end u \<Longrightarrow>
+   HL_COREC_term u = Lam x t"
+  unfolding HL_COREC_term_def Lam_def
+  apply (subst HL_to_LL.COREC_dtor[of "Abs_term_pre (Inr (Inr (x, Inl t)))"])
+    apply (subst Udtor_Udlam_stop, assumption+)
+    apply (rule image_eqI[of _ _ "(x, t)"])
+     apply (unfold prod.case)
+     apply (rule refl)
+    apply assumption+
+  apply (unfold term_pre_map_simps)
+  apply (rule refl)
+  done
+
+lemma HL_COREC_term_Lam_cont:
+  "validU u \<Longrightarrow> is_Udlam u \<Longrightarrow> \<not> Udlam_stop u \<Longrightarrow> (x, u') \<in> Udlam_cont u \<Longrightarrow>
+   HL_COREC_term u = Lam x (HL_COREC_term u')"
+  unfolding HL_COREC_term_def Lam_def
+  apply (subst HL_to_LL.COREC_dtor[of "Abs_term_pre (Inr (Inr (x, Inr u')))"])
+    apply (subst Udtor_Udlam_cont, assumption+)
+    apply (rule image_eqI[of _ _ "(x, u')"])
+     apply (unfold prod.case)
+     apply (rule refl)
+    apply assumption+
+  apply (unfold term_pre_map_simps)
+  apply (rule refl)
+  done
+
+lemmas HL_COREC_term_swap   = HL_to_LL.COREC_swap[folded HL_COREC_term_def]
+lemmas HL_COREC_term_UFVars = HL_to_LL.COREC_FVars[folded HL_COREC_term_def]
+lemmas HL_COREC_term_dtor   = HL_to_LL.COREC_dtor[folded HL_COREC_term_def]
+
+end
+
+interpretation const_HL: HL_COREC_term
+  where
+        Umap        = "image :: ('a :: covar \<Rightarrow> 'a) \<Rightarrow> 'a set \<Rightarrow> 'a set"
+    and UFVars      = "id :: 'a :: covar set \<Rightarrow> 'a set"
+    and validU      = "finite :: 'a :: covar set \<Rightarrow> bool"
+    and is_Udvar    = "\<lambda>_. False"
+    and Udvar       = "\<lambda>_. undefined"
+    and is_Udapp    = "\<lambda>_. False"
+    and Udapp_stop1 = "\<lambda>_. undefined"
+    and Udapp_end1  = "\<lambda>_. undefined"
+    and Udapp_cont1 = "\<lambda>_. undefined"
+    and Udapp_stop2 = "\<lambda>_. undefined"
+    and Udapp_end2  = "\<lambda>_. undefined"
+    and Udapp_cont2 = "\<lambda>_. undefined"
+    and is_Udlam    = "\<lambda>_. True"
+    and Udlam_stop  = "\<lambda>_. False"
+    and Udlam_end   = "\<lambda>_. {}"
+    and Udlam_cont  = "\<lambda>A. {(z, insert z A) | z. z \<notin> A}"
+  apply unfold_locales
+                      apply (simp_all add: arb_element image_image)
+  subgoal for A x x'
+    apply (rule exI[where x="swap x x'"])
+    apply (auto simp: id_on_def)
+      apply (metis swap_simps(3))
+     apply (metis swap_simps(3))
+    apply (metis image_iff swap_simps(3))
+    done
+  subgoal for A f
+    apply (rule set_eqI, auto simp: image_iff bij_inv_eq_iff)
+     subgoal for z by (rule exI[where x="inv f z"]) (auto simp: bij_inv_eq_iff)
+    by (metis bij_betw_imp_inj_on inj_eq)
+  done
+
+lemma "finite A \<Longrightarrow> z \<notin> A \<Longrightarrow>
+  const_HL.HL_COREC_term A = Lam z (const_HL.HL_COREC_term (insert z A))"
+  by (subst const_HL.HL_COREC_term_Lam_cont[where x=z and u'="insert z A"]) auto
 
 end
