case_studies/Untyped_Lambda_Calculus/LC_HL_LL_REC_Examples.thy
@@ -1,0 +1,87 @@
+theory LC_HL_LL_REC_Examples
+  imports LC
+begin
+
+context begin
+
+interpretation subst_inst: HL_REC_term
+  where
+      Pmap         = "\<lambda>f (x :: 'a :: var, s). (f x, permute_term f s)"
+  and PFVars       = "\<lambda>(x :: 'a :: var, s). {x} \<union> FFVars s"
+  and validP       = "\<lambda>(x :: 'a :: var, s). True"
+  and avoiding_set = "{}"
+  and Umap         = "\<lambda>f t r. permute_term f r"
+  and UFVars       = "\<lambda>t r. FFVars r"
+  and validU       = "\<lambda>r. True"
+  and UVar         = "\<lambda>y (x, s). if y = x then s else Var y"
+  and UApp         = "\<lambda>t1 pu1 t2 pu2 p. App (pu1 p) (pu2 p)"
+  and ULam         = "\<lambda>y t pu p. Lam y (pu p)"
+  apply standard
+  apply (auto simp: term.permute_comp inj_eq
+              intro!: term.Un_bound singl_bound term.set_bd_UNIV emp_bound
+                      term.permute_cong_id
+              split: if_splits prod.splits
+              dest: bij_is_inj)
+  apply blast
+  done
+
+definition "subst x s t = subst_inst.HL_REC_term t (x, s)"
+
+lemmas subst_simps[where p = "(x, s)" for x s, folded subst_def, simplified] =
+  subst_inst.HL_REC_term_Var
+  subst_inst.HL_REC_term_App
+  subst_inst.HL_REC_term_Lam
+end
+
+schematic_goal subst_eval:
+  "y \<noteq> x \<Longrightarrow> y \<noteq> z \<Longrightarrow>
+   subst x (Var z) (App (Var x) (Lam y (Var x))) = ?t"
+  by (simp add: subst_simps)
+
+
+context begin
+
+interpretation subst_LL_inst: REC_term
+  where
+      Pmap         = "\<lambda>f (x :: 'a :: var, s). (f x, permute_term f s)"
+  and PFVars       = "\<lambda>(x :: 'a :: var, s). {x} \<union> FFVars s"
+  and validP       = "\<lambda>(x :: 'a :: var, s). True"
+  and avoiding_set = "{}"
+  and Umap         = "\<lambda>f t r. permute_term f r"
+  and UFVars       = "\<lambda>t r. FFVars r"
+  and validU       = "\<lambda>r. True"
+  and Uctor        = "\<lambda>x' (xp, sp). (case Rep_term_pre x' of
+      Inl y                            \<Rightarrow> (if y = xp then sp else Var y)
+    | Inr (Inl ((_, pu1), (_, pu2)))   \<Rightarrow> App (pu1 (xp, sp)) (pu2 (xp, sp))
+    | Inr (Inr (y, _, pu))             \<Rightarrow> Lam y (pu (xp, sp)))"
+  apply unfold_locales
+              apply (auto simp: term.permute_comp
+                          intro!: term.Un_bound singl_bound term.set_bd_UNIV emp_bound
+                                  term.permute_cong_id)
+  subgoal for f y p
+    apply (tactic \<open>resolve_tac @{context}
+      [BNF_FP_Util.mk_absumprodE @{thm type_definition_term_pre} [1, 2, 2]
+       |> infer_instantiate' @{context} [SOME (Thm.cterm_of @{context} @{term y})]] 1\<close>)
+    apply (auto simp: Abs_term_pre_inverse[OF UNIV_I] map_term_pre_def comp_def
+                      term.permute_inv_simp[symmetric] term.permute_bij inj_eq
+                dest: bij_is_inj)
+    done
+  subgoal for p y
+    apply (tactic \<open>resolve_tac @{context}
+      [BNF_FP_Util.mk_absumprodE @{thm type_definition_term_pre} [1, 2, 2]
+       |> infer_instantiate' @{context} [SOME (Thm.cterm_of @{context} @{term p})]] 1\<close>)
+    apply hypsubst_thin
+    apply (auto simp: Abs_term_pre_inverse[OF UNIV_I] map_term_pre_def comp_def
+                      Var_def[symmetric] App_def[symmetric] Lam_def[symmetric]
+                      set2_term_pre_def set3_term_pre_def set4_term_pre_def
+                split: if_splits)
+    apply blast+
+    done
+  done
+
+definition "subst_LL x s t = subst_LL_inst.REC_term t (x, s)"
+
+end
+
+
+end
